ulib/LowStar.RST.NonScoped.fst
@@ -1,0 +1,190 @@
+(*
+   Copyright 2008-2019 Microsoft Research
+
+   Licensed under the Apache License, Version 2.0 (the "License");
+   you may not use this file except in compliance with the License.
+   You may obtain a copy of the License at
+
+       http://www.apache.org/licenses/LICENSE-2.0
+
+   Unless required by applicable law or agreed to in writing, software
+   distributed under the License is distributed on an "AS IS" BASIS,
+   WITHOUT WARRANTIES OR CONDITIONS OF ANY KIND, either express or implied.
+   See the License for the specific language governing permissions and
+   limitations under the License.
+*)
+module LowStar.RST.NonScoped
+
+open FStar.HyperStack.ST
+module B = LowStar.Buffer
+module HS = FStar.HyperStack
+module HST = FStar.HyperStack.ST
+
+open LowStar.Resource
+
+(* Additional (currently assumed) lemma: 
+     Reasonable when addresses are not reused after deallocation, 
+     but currently not provided by the LowStar.Buffer library
+     (Nik and/or Tahina will look into adding it to ulib) *)
+(*assume val lemma_loc_not_unused_in_modifies (l:B.loc) (h0 h1:HS.mem)
+  : Lemma (requires (B.loc_includes (B.loc_not_unused_in h0) l /\ B.modifies l h0 h1))
+          (ensures  (B.loc_includes (B.loc_not_unused_in h1) l))*)
+
+assume val lemma_loc_not_unused_in_modifies_includes (l0 l1:B.loc) (h0 h1:HS.mem)
+  : Lemma (requires (B.loc_includes (B.loc_not_unused_in h0) l0 /\ 
+                     B.loc_includes l1 l0 /\
+                     B.modifies l1 h0 h1))
+          (ensures  (B.loc_includes (B.loc_not_unused_in h1) l1))
+
+(* Abstract modifies clause for the resource-indexed state effect *)
+
+abstract
+let modifies (res:resource) (h0 h1:HS.mem) =
+    B.modifies (as_loc (fp res)) h0 h1 // /\
+    //HST.equal_domains h0 h1
+
+let modifies_refl (res:resource) (h:HS.mem) 
+  : Lemma (modifies res h h)
+           [SMTPat (modifies res h h)]
+  = ()
+
+let modifies_trans (res0 res1:resource) (h0 h1 h2:HS.mem) 
+  : Lemma (requires 
+             modifies res0 h0 h1 /\
+             modifies res1 h1 h2)
+           (ensures
+             modifies (r_union res0 res1) h0 h2)
+           [SMTPat (modifies (r_union res0 res1) h0 h2);
+            SMTPat (modifies res0 h0 h1)]
+  = ()
+
+let reveal_modifies ()
+  : Lemma (forall res h0 h1.{:pattern modifies res h0 h1}
+             modifies res h0 h1 <==>
+             B.modifies (as_loc (fp res)) h0 h1) // /\
+             //HST.equal_domains h0 h1)
+  = ()
+
+(* State effect indexed by resources *)
+
+let r_pre (res:resource) = imem (inv res) -> Type0
+let r_post res0 a res1 = imem (inv res0) -> x:a -> imem (inv (res1 x)) -> Type0
+
+abstract
+let rst_inv (res:resource) (h:HS.mem) =
+  B.loc_includes (B.loc_not_unused_in h) (as_loc (fp res))
+
+let reveal_rst_inv ()
+  : Lemma (forall res h . 
+             rst_inv res h 
+             <==>
+             B.loc_includes (B.loc_not_unused_in h) (as_loc (fp res)))
+  = ()
+
+let prov_resource res0 =
+  res1:resource{(forall frame . r_disjoint frame res0 ==> r_disjoint frame res1)}
+
+effect RST (a:Type)
+           (res0:resource)                                      //Resources expected
+           (res1:a -> prov_resource res0)                       //Resources provided
+           (pre:r_pre res0)
+           (post:r_post res0 a res1) = 
+       STATE a
+            (fun (k:a -> HS.mem -> Type)
+               (h0:HS.mem) ->
+               inv res0 h0 /\                                    //Require the resource invariant
+               rst_inv res0 h0 /\                                //Require the additional footprints invariant
+               pre h0 /\                                         //Require the pre-condition
+               (forall (x:a) (h1:HS.mem).
+                 inv (res1 x) h1 /\                              //Ensure the resource invariant
+                 rst_inv (res1 x) h1 /\                          //Ensure the additional footprints invariant
+                 modifies (r_union res0 (res1 x)) h0 h1 /\       //Ensure that only resource's footprint is modified
+                 post h0 x h1 ==>                                //Ensure the post-condition
+                 k x h1))                                         //Prove the continuation under this hypothesis
+
+(* Generic frame operation for RST computations (through resource inclusion) *)
+
+unfold
+let frame_pre (frame:resource)
+              (#fp:resource)
+              (pre:r_pre fp)
+              (h:imem (inv (frame <*> fp))) =
+  pre h
+
+unfold
+let frame_post (frame:resource)
+               (#fp0:resource)
+               (#a:Type)
+               (#fp1:a -> prov_resource fp0)
+               (post:r_post fp0 a fp1)
+               (h0:imem (inv (frame <*> fp0)))
+               (x:a)
+               (h1:imem (inv (frame <*> fp1 x))) = 
+  post h0 x h1 /\
+  sel (view_of frame) h0 == sel (view_of frame) h1
+
+let frame (#frame:resource)
+          (#fp0:resource)
+          (#a:Type)
+          (#fp1:a -> prov_resource fp0)
+          (#pre:r_pre fp0)
+          (#post:r_post fp0 a fp1)
+          ($f:unit -> RST a fp0 fp1 pre post)
+        : RST a (frame <*> fp0) 
+                (fun x -> reveal_star (); frame <*> fp1 x) 
+                (frame_pre frame pre) 
+                (frame_post frame post) =
+  reveal_view ();
+  reveal_star ();
+  let h0 = get () in 
+  let x = f () in 
+  let h1 = get () in 
+  lemma_loc_not_unused_in_modifies_includes 
+    (as_loc (fp (frame <*> fp0))) 
+    (as_loc (fp (r_union (frame <*> fp0) (frame <*> fp1 x)))) 
+    h0 h1;
+  x
+
+
+unfold
+let weaken_pre (#outer0:resource)
+               (#inner0:resource)
+               (delta0:r_includes outer0 inner0)
+               (pre:r_pre inner0)
+               (h:imem (inv outer0)) =
+  pre h
+
+unfold
+let weaken_post (#outer0:resource)
+                (#inner0:resource)
+                (#a:Type)
+                (#outer1:a -> prov_resource outer0)
+                (#inner1:a -> prov_resource inner0)
+                (delta0:r_includes outer0 inner0)
+                (delta1:(x:a -> r_includes (outer1 x) (inner1 x)))
+                (post:r_post inner0 a inner1)
+                (h0:imem (inv outer0))
+                (x:a)
+                (h1:imem (inv (outer1 x))) = 
+  assert (inv (outer1 x) h1 ==> inv (delta1 x) h1); // needed to trigger (inv (outer1 x) h1 ==> inv (inner1 x) h1) from (delta1 x)
+  post h0 x h1 /\
+  sel (view_of delta0) h0 === sel (view_of (delta1 x)) h1 // only makes sense if the deltas have the views with same types
+
+let weaken (#outer0:resource)
+           (#inner0:resource)
+           (#a:Type)
+           (#outer1:a -> prov_resource outer0)
+           (#inner1:a -> prov_resource inner0)
+           (delta0:r_includes outer0 inner0)
+           (delta1:(x:a -> r_includes (outer1 x) (inner1 x)))
+           (#pre:r_pre inner0)
+           (#post:r_post inner0 a inner1)
+           ($f:unit -> RST a inner0 inner1 pre post)
+         : RST a outer0 outer1 (weaken_pre delta0 pre) 
+                               (weaken_post delta0 delta1 post) =
+  reveal_view ();
+  let h0 = get () in 
+  let x = f () in 
+  let h1 = get () in 
+  assert (inv (inner1 x) h1);
+  admit ()
